\documentclass{article}
\usepackage{fullpage}
\usepackage{nopageno}
\usepackage{amsmath}

\setlength{\parindent}{0pt}
\setlength{\parskip}{.2in}

\begin{document}

Proof by induction that
\[ \sum_{i=0}^{n}{i^2} = \frac{n(n+1)(2n+1)}{6} \] for all integers $n \ge 1$.

{\bf Induction hypothesis}: The general case of the induction hypothesis, $IH(n)$, is
\[ f(n) = \sum_{i=0}^{n}{i^2} = \frac{n(n+1)(2n+1)}{6} \]

{\bf Basis step}: $IH(1)$ predicts that
\[ f(1) = \sum_{i=0}^{1}{i^2} = \frac{1(1+1)(2\cdot 1+1)}{6} = \frac{1\cdot 2\cdot 3}{6} = \frac{6}{6} = 1 \]
This is the sum of the squares from 0 to 1, so $IH(1)$ is true.

{\bf Induction step}:

Expectation: $IH(n+1)$ is
\[ f(n+1) = \sum_{i=0}^{n+1}{i^2} = \frac{(n+1)(n+2)(2(n+1)+1)}{6} \]

Connecting cases for $n$ and $n+1$: we can observe that
\begin{alignat*}{2}
f(n+1) = \sum_{i=0}^{n+1}{i^2} &= 1^2 + 2^2 + 3^3 + \ldots + n^2 + (n+1)^2 \\
                               &= \sum_{i=0}^{n}{i^2} + (n+1)^2 \\
                               &= f(n) + (n+1)^2
\end{alignat*}

Assuming $IH(n)$ is true, then
\begin{alignat*}{2}
f(n+1) &= f(n) + (n+1)^2 \\
       &= \frac{n(n+1)(2n+1)}{6} + (n+1)^2 \\
       &= \frac{2n^3 + 9n^2 + 13n + 6}{6} \\
       &= \frac{(n+1)(n+2)(2(n+1)+1)}{6}
\end{alignat*}

This matches the expectation, proving that if $IH(n)$ is true, then $IH(n+1)$ must also
be true.

\end{document}
